examples/alethe-tests.v
@@ -32,6 +32,7 @@ Local Open Scope int63_scope.
 
 Section Checker_SmtEx.
   Parse_certif_verit t_i0 t_func0 t_atom0 t_form0 root0 used_roots0 trace0 "/home/arjun/Desktop/smtcoq/arjunvish-smtcoq-veritparser/smtcoq/examples/verit_coq8f5ac2.smt2" "/home/arjun/Desktop/smtcoq/arjunvish-smtcoq-veritparser/smtcoq/examples/verit_coq8f5ac2.vtlog".
+  (*Eval compute in (Form.check_form t_form0 && Atom.check_atom t_atom0 && Atom.wt t_i0 t_func0 t_atom0).*)
 End Checker_SmtEx.
 
 Goal negb (true && (negb true)).
